programs/Cholesky.fst
@@ -7,9 +7,9 @@ let rec cholesky (#n:pos) (m:mat n{spd m}) :
   match m with
   | Mat1 a -> 
     Mat1 (sqrt a)
-  | MatN d c a b ->
+  | MatN _ c a _ ->
       let l11 = sqrt a in
       let l21 = vec_scalar_div c l11 in
-      let s = schur1 d c a b in
+      let s = schur1 m in
       let l = cholesky s in
       MatN l l21 l11 zero_rvec
